lean/AbsDen.lean
@@ -4,6 +4,8 @@ import AbsDen.World.DeriveTests
 import AbsDen.Env
 import AbsDen.Semantics
 import AbsDen.Trace
+import AbsDen.LR
 import AbsDen.ByName
 import AbsDen.ByNeed
 import AbsDen.NoConsecInvis
+import AbsDen.LRGood
